Java/src/Java/Func/Reify.v
@@ -8,8 +8,8 @@ Require Import MirrorCore.Lib.ApplicativeView.
 Require Import MirrorCore.Lib.ProdView.
 Require Import MirrorCore.Lib.EqView.
 Require Import MirrorCore.Lib.NatView.
-Require Import MirrorCore.Lib.BoolView.
 Require Import MirrorCore.Lib.StringView.
+Require Import MirrorCore.Lib.BoolView.
 Require Import MirrorCore.Lib.ProdView.
 Require Import MirrorCore.CTypes.CoreTypes.
 Require Import MirrorCore.CTypes.BaseType.
@@ -30,6 +30,10 @@ Require Import Charge.Views.BILogicView.
 Require Import Charge.Views.EmbedView.
 Require Import Charge.Views.SubstView.
 
+Require Import Charge.Reify.ILogicReify.
+Require Import Charge.Reify.BILogicReify.
+Require Import Charge.Reify.EmbedReify.
+
 Require Import ChargeCore.Open.Stack.
 Require Import ChargeCore.Open.Subst.
 Require Import ChargeCore.Open.OpenILogic.
@@ -39,7 +43,6 @@ Require Import ChargeCore.Logics.Later.
 
 Require Import ExtLib.Structures.Applicative.
 Require Import MirrorCore.Lib.NatView.
-
 
 Reify Declare Typed Table term_table : BinNums.positive => typ.
 
@@ -52,19 +55,19 @@ Global Instance Reify_typ : Reify typ :=
   Reify_typ typ (reify_base_typ typ ::
                  reify_list_typ typ ::
                  reify_prod_typ typ ::
-                 reify_subst_typ typ _ String.string val ::
+                 reify_subst_typ typ _ Lang.var val ::
                  reify_java_typ typ :: nil).
 
 Global Instance Reify_java : Reify (expr typ func) :=
-  Reify_func typ func term_table (reify_java_func ::
+  Reify_func typ func (reify_java_func ::
                                   reify_nat typ func ::
                                   reify_bool typ func ::
-                                  reify_string typ func :: 
                                   reify_eq typ func ::
-                                  reify_applicative typ func (RFun (RFun String.string val)) ::
+                                  reify_applicative typ func (RFun (String.string -> val)) ::
                                   reify_list typ func :: 
                                   reify_listOp typ func :: 
                                   reify_prod typ func ::
+                                  reify_string typ func ::
           	                  reify_ilogic typ func :: 
           	                  reify_plogic typ func :: 
                                   reify_bilogic typ func ::
@@ -84,6 +87,19 @@ Ltac reify_java e :=
              [[ (fun (y : @mk_dvar_map _ _ _ _ term_table elem_ctor) => True) ]]
              [[ e ]].
 
+Local Instance fs : Environment := 
+  Build_Environment (FMapPositive.PositiveMap.empty (SymEnv.function typ _)).
+
+Ltac reify_java_debug e :=
+  let n := fresh "n" in
+  let k fs e :=
+      pose e as n in
+  reify_expr reify_java k
+             [[ (fun (y : @mk_dvar_map _ _ _ _ term_table elem_ctor) => True) ]]
+             [[ e ]];
+  let t := eval cbv in (@typeof_expr typ func RType_typ _ RSym_func nil nil n) in
+                          idtac t.
+
 Ltac reify_typ e :=
   let k fs e :=
       pose e in
@@ -92,84 +108,108 @@ Ltac reify_typ e :=
              [[ e ]].
 
 Notation "'ap_eq' '[' x ',' y ']'" :=
-	 (ap (T := RFun (RFun String.string val)) (ap (T := RFun (RFun String.string val)) (pure (T := RFun (RFun String.string val)) (@eq val)) x) y).
+	 (ap (T := RFun (String.string -> val)) (ap (T := RFun (String.string -> val)) (pure (T := RFun (String.string -> val)) (@eq val)) x) y).
 Notation "'ap_pointsto' '[' x ',' f ',' e ']'" :=
-	(ap (T := RFun (RFun String.string val)) (ap (T := RFun (RFun String.string val)) (ap (T := RFun (RFun String.string val))
-		(pure (T := RFun (RFun String.string val)) pointsto) (stack_get x))
-			(pure (T := RFun (RFun String.string val)) f)) e).
+	(ap (T := RFun (String.string -> val)) (ap (T := RFun (String.string -> val)) (ap (T := RFun (String.string -> val))
+		(pure (T := RFun (String.string -> val)) pointsto) (stack_get x))
+			(pure (T := RFun (String.string -> val)) f)) e).
 Notation "'ap_typeof' '[' e ',' C ']'" :=
-	(ap (T := RFun (RFun String.string val))
-	    (ap (T := RFun (RFun String.string val))
-	        (pure (T := RFun (RFun String.string val)) typeof)
-	        (pure (T := RFun (RFun String.string val)) C))
+	(ap (T := RFun (String.string -> val))
+	    (ap (T := RFun (String.string -> val))
+	        (pure (T := RFun (String.string -> val)) typeof)
+	        (pure (T := RFun (String.string -> val)) C))
 	    e).
 
-Goal (forall (Pr : Program) (C : class) (v : val) (x f : String.string) (fields : list field) (ex : (RFun (RFun String.string val) val)), True).
+
+Goal (forall (Pr : Program) (C : class) (v : val) (x : String.string) (f : field) (fields : list field) (ex : (RFun (String.string -> val) val)), True).
   intros Pr C v x f fields ex.
-  reify_java 5.
-  reify_java (typeof C v).
-  reify_java (field_lookup).
-  reify_java (5::4::3::@nil nat).
-  reify_java (field_lookup Pr C fields).
-  reify_java True.
-  reify_java False.
-  reify_java (True \/ False).
-  reify_java (True /\ False).
-  reify_java (False -> True).
-  reify_java (5 = 5).
-  reify_java (exists x, x = 5).
-  reify_java (forall x, x = 5).
+  reify_java_debug 5.
+  reify_java_debug (typeof C v).
+  reify_java_debug (field_lookup).
+  reify_java_debug (5::4::3::@nil nat).
+  reify_java_debug (field_lookup Pr C fields).
+  reify_java_debug True.
+  reify_java_debug False.
+  reify_java_debug (True \/ False).
+  reify_java_debug (True /\ False).
+  reify_java_debug (False -> True).
+  reify_java_debug (5 = 5).
+  reify_java_debug (exists x, x = 5).
+  reify_java_debug (forall x, x = 5).
 
-  reify_java (ap (T := RFun (RFun String.string val)) (ap (T := RFun (RFun String.string val)) (pure (T := RFun (RFun String.string val)) pointsto) (stack_get x)) (pure (T := RFun (RFun String.string val)) x)).
+  reify_java_debug (stack_get (val := val) x).
+  reify_java_debug (pure (T := RFun (String.string -> val)) pointsto).
+  reify_java_debug (Applicative.pure (T := RFun (String.string -> val)) 5).
+  reify_typ Lang.var.
 
-  reify_java (fun a b c => pointsto a b c).
+  reify_java_debug (ap (T := RFun (String.string -> val))
+                     (pure (T := RFun (String.string -> val)) pointsto)
+                     (stack_get (val := val) x)).
+
+  reify_java_debug (ap (T := RFun (String.string -> val)) 
+                       (ap (T := RFun (String.string -> val)) 
+                           (pure (T := RFun (String.string -> val)) pointsto) 
+                     (stack_get x)) 
+                 (pure (T := RFun (String.string -> val)) f)).
+
+  reify_java_debug (fun a b c => pointsto a b c).
 
 
   pose (E_val (vint 3)) as d.
 
-  reify_java (pure (T := RFun (RFun String.string val)) (vbool true)).
+  reify_java_debug (pure (T := RFun (String.string -> val)) (vbool true)).
 
-  reify_java (forall x : nat, x = x).
-Check @pure.
-  reify_java (ap (T := RFun (RFun String.string val)) (pure (T := RFun (RFun String.string val)) (@eq val)) (eval d)).
+  reify_java_debug (forall x : nat, x = x).
 
-  reify_java (ap_pointsto [x, x, (eval d)]).
+  reify_java_debug (ap (T := RFun (String.string -> val)) (pure (T := RFun (String.string -> val)) (@eq val)) (eval d)).
+
+  reify_java_debug (ap_pointsto [x, f, (eval d)]).
 
   generalize String.EmptyString. intro c.
-  reify_java (cread c c c).
+  reify_java_debug (cread c c c).
 
-   reify_java (ltrue |-- triple ltrue ltrue (cread c c c)).
-   reify_java (ltrue |-- {[ ltrue ]} cread c c c {[ ltrue ]}).
+   reify_java_debug (ltrue |-- triple ltrue ltrue (cread c c c)).
+   reify_java_debug (ltrue |-- {[ ltrue ]} cread c c c {[ ltrue ]}).
 
-  reify_java cskip.
+  reify_java_debug cskip.
 
-  reify_java (forall P, P /\ P).
+  reify_java_debug (forall P, P /\ P).
 
-  reify_java (forall x : nat, x = x).
-  reify_java (exists x : nat, x = x).
+  reify_java_debug (forall x : nat, x = x).
+  reify_java_debug (exists x : nat, x = x).
 
-  reify_java (@subst1 String.string val _).
-  reify_java (cseq cskip cskip).
+  reify_java_debug (@subst1 String.string val _).
+  reify_java_debug (cseq cskip cskip).
 
-  reify_java (@map nat nat).
-  reify_java (ILogic.lentails True True).
+  reify_java_debug (@map nat nat).
+  reify_java_debug (ILogic.lentails True True).
 
-  reify_java ((True -> False) -> True).
-  reify_java (forall P Q, P /\ Q).
+  reify_java_debug ((True -> False) -> True).
+  reify_java_debug (forall P Q, P /\ Q).
 
-  reify_java (forall P : sasn, ILogic.lentails ILogic.ltrue P).
-  reify_java (forall (G : spec) (P Q : sasn), ILogic.lentails G (triple P Q cskip)).
+  reify_java_debug (forall P : sasn, ILogic.lentails ILogic.ltrue P).
+  reify_java_debug (forall (G : spec) (P Q : sasn), ILogic.lentails G (triple P Q cskip)).
   generalize (String.EmptyString : String.string).
   intro y.
 
-  reify_java (stack_get (A := String.string) (val := val)).
-  reify_java (@stack_get String.string val y).
+  reify_java_debug (stack_get (A := String.string) (val := val)).
+  reify_java_debug (@stack_get String.string val y).
 
-  reify_java (stack_get (val := val) y).
+  reify_java_debug (stack_get (val := val) x).
 
-  reify_java (y = y).
+  reify_java_debug (y = y).
 
-  reify_java (@ltrue sasn _).
+  reify_java_debug (@ltrue sasn _).
+
+  reify_java_debug (eval (E_not (E_val v))).
+  reify_java_debug (pure (T := RFun (String.string -> val)) (vbool true)).
+
+Require Import ChargeCore.Logics.ILEmbed.
+
+  reify_java_debug
+    (@embed ((String.string -> val) -> Prop) sasn _ 
+            (ap_eq [eval (E_not (E_val v)), pure (vbool true)]) //\\ ltrue).
+  
 
   exact I.
 
